## 1.次の微分方程式の一般解を求めよ

> [!note] (e)
> $$
>     y^{\prime} - 2y = -2y^2
> $$

> [!success]- (e) 解答
> $$
>     \begin{align}
>         y^{\prime} - 2y & = -2y^2 \\
>         y^{\prime} & = 2y(1-y) \\
>         \frac{dy}{2y(1-y)} & = dx \\
>         \int \frac{dy}{2y(1-y)} & = \int dx \\
>         \frac{1}{2} \int \left( \frac{1}{y} + \frac{1}{1-y} \right) dy & = x + C \\
>         \frac{1}{2} \left( \log y - \log (1-y) \right) & = x + C \\
>         \log \frac{y}{1-y} & = 2x + C \\
>         \frac{y}{1-y} & = e^{2x + C} \\
>         y & = (1-y)e^{2x + C} \\
>         y & = e^{2x + C} - ye^{2x + C} \\
>         y + ye^{2x + C} & = e^{2x + C} \\
>         y(1 + e^{2x + C}) & = e^{2x + C} \\
>         y & = \frac{e^{2x + C}}{1 + e^{2x + C}} \\
>         y & = \frac{1}{e^{-2x - C} + 1} \\
>         y & = \frac{1}{C^{\prime}e^{-2x} + 1} \\
>     \end{align}
> $$
